Benchmarks/FluxRS/FibTwelve.lean
@@ -1,3 +1,5 @@
+import LeanFixpoint
+
 @[simp]
 def fib_spec_twelve : Int := 12
 
@@ -5,5 +7,4 @@ def FibTwelve :=
  ((3 + 9) = (fib_spec_twelve))
 
 def FibTwelve_proof : FibTwelve := by
-  unfold FibTwelve
-  simp
+  solve_fixpoint
