LeanFixpoint/Tactic/SolveFixpoint.lean
@@ -77,7 +77,7 @@ private def closeResidualGoals : TacticM Unit := do
   let goals ← getGoals
   if goals.isEmpty then pure ()
   else
-    let _ ← attemptTactic (evalTactic (← `(tactic| simp_all)))
+    let _ ← attemptTactic (evalTactic (← `(tactic| simp only [])))
     let goals ← getGoals
     if goals.isEmpty then pure ()
     else closeLoop
@@ -156,11 +156,12 @@ private def solveFixpointImpl (qs? : Option (TSyntax `term)) : TacticM Unit := w
       logInfo m!"[solve_fixpoint] Cyclic:  {cyclic.map (·.name)}"
 
       -- Phase 2: Fusion - eliminate acyclic κ-vars
-      let mut solutions : List (Name × Pred) := []
+      -- solutions need name of κ, solution pred and list of κ formal params
+      let mut solutions : List (Name × Pred × List Name) := []
       let mut curr := constraint
       for κ in acyclic do
         let sol := curr.sol1 κ
-        solutions := solutions ++ [(κ.name, sol)]
+        solutions := solutions ++ [(κ.name, sol, κ.params)]
         curr := curr.elim1 κ
 
       for (κName, sol) in solutions do
@@ -173,15 +174,15 @@ private def solveFixpointImpl (qs? : Option (TSyntax `term)) : TacticM Unit := w
           let pa ← predicateAbstraction curr Q
           for (κ, qs) in pa do
             let sol   := conjoinQualifiers qs
-            solutions := solutions ++ [(κ.name, sol)]
+            solutions := solutions ++ [(κ.name, sol, κ.params)]
             curr      := curr.elimStar κ sol
         | none   => logWarning m!"[solve_fixpoint] Cyclic κ-vars present but no qualifiers provided"
 
       -- NOTE: One may need to be careful with order of instantiations
       -- Phase 4: Witness synthesis for acyclic solutions
-      for (_κName, sol) in solutions do
+      for (_κName, sol, params) in solutions do
         logInfo m!"[solve_fixpoint] Elaborating witness for: {toString sol}"
-        let witness    ← solToWitnessExpr sol
+        let witness    ← solToWitnessExpr sol params
         let witnessSyn ← PrettyPrinter.delab witness
         evalTactic (← `(tactic| refine ⟨$witnessSyn, ?_⟩))
     )
